Update execution layer with new contract signature

execution/test/LocalBlockchain.v
@@ -22,498 +22,520 @@ From Coq Require Import Psatz.
 Import ListNotations.
 
 Section LocalBlockchain.
-Local Open Scope bool.
+  Local Open Scope bool.
 
-Context {AddrSize : N}.
-Context {DepthFirst : bool}.
+  Context {AddrSize : N}.
+  Context {DepthFirst : bool}.
 
-Definition ContractAddrBase : N := AddrSize / 2.
+  Definition ContractAddrBase : N := AddrSize / 2.
 
-Global Instance LocalChainBase : ChainBase :=
-  {| Address := BoundedN AddrSize;
-     address_eqb := BoundedN.eqb;
-     address_eqb_spec := BoundedN.eqb_spec;
-     address_is_contract a := (ContractAddrBase <=? BoundedN.to_N a)%N
-  |}.
+  Global Instance LocalChainBase : ChainBase :=
+    {| Address := BoundedN AddrSize;
+      address_eqb := BoundedN.eqb;
+      address_eqb_spec := BoundedN.eqb_spec;
+      address_is_contract a := (ContractAddrBase <=? BoundedN.to_N a)%N
+    |}.
 
-Record LocalChain :=
-  build_local_chain {
-    lc_height : nat;
-    lc_slot : nat;
-    lc_fin_height : nat;
-    lc_account_balances : FMap Address Amount;
-    lc_contract_state : FMap Address SerializedValue;
-    lc_contracts : FMap Address WeakContract;
-  }.
+  Record LocalChain :=
+    build_local_chain {
+      lc_height : nat;
+      lc_slot : nat;
+      lc_fin_height : nat;
+      lc_account_balances : FMap Address Amount;
+      lc_contract_state : FMap Address SerializedValue;
+      lc_contracts : FMap Address WeakContract;
+    }.
 
-MetaCoq Run (make_setters LocalChain).
+  MetaCoq Run (make_setters LocalChain).
 
-Definition lc_to_env (lc : LocalChain) : Environment :=
-  {| env_chain :=
-        {| chain_height := lc_height lc;
-           current_slot := lc_slot lc;
-           finalized_height := lc_fin_height lc; |};
-     env_account_balances a := with_default 0%Z (FMap.find a (lc_account_balances lc));
-     env_contract_states a := FMap.find a (lc_contract_state lc);
-     env_contracts a := FMap.find a (lc_contracts lc); |}.
+  Definition lc_to_env (lc : LocalChain) : Environment :=
+    {| env_chain :=
+          {| chain_height := lc_height lc;
+            current_slot := lc_slot lc;
+            finalized_height := lc_fin_height lc; |};
+      env_account_balances a := with_default 0%Z (FMap.find a (lc_account_balances lc));
+      env_contract_states a := FMap.find a (lc_contract_state lc);
+      env_contracts a := FMap.find a (lc_contracts lc); |}.
 
-Global Coercion lc_to_env : LocalChain >-> Environment.
+  Global Coercion lc_to_env : LocalChain >-> Environment.
 
-Section ExecuteActions.
-  Local Open Scope Z.
+  Section ExecuteActions.
+    Local Open Scope Z.
 
-  Definition add_balance (addr : Address) (amt : Amount) (lc : LocalChain) : LocalChain :=
-    let update opt := Some (amt + with_default 0 opt) in
-    lc<|lc_account_balances ::= FMap.partial_alter update addr|>.
+    Definition add_balance
+                (addr : Address)
+                (amt : Amount)
+                (lc : LocalChain)
+                : LocalChain :=
+      let update opt := Some (amt + with_default 0 opt) in
+      lc<|lc_account_balances ::= FMap.partial_alter update addr|>.
 
-  Definition transfer_balance
-            (from to : Address) (amount : Amount) (lc : LocalChain) : LocalChain :=
-    add_balance to amount (add_balance from (-amount) lc).
+    Definition transfer_balance
+                (from to : Address)
+                (amount : Amount)
+                (lc : LocalChain)
+                : LocalChain :=
+      add_balance to amount (add_balance from (-amount) lc).
 
-  Definition get_new_contract_addr (lc : LocalChain) : option Address :=
-    BoundedN.of_N (ContractAddrBase + N.of_nat (FMap.size (lc_contracts lc))).
+    Definition get_new_contract_addr (lc : LocalChain) : option Address :=
+      BoundedN.of_N (ContractAddrBase + N.of_nat (FMap.size (lc_contracts lc))).
 
-  Definition add_contract
-             (addr : Address)
-             (wc : WeakContract)
-             (lc : LocalChain) : LocalChain :=
-    lc<|lc_contracts ::= FMap.add addr wc|>.
+    Definition add_contract
+                (addr : Address)
+                (wc : WeakContract)
+                (lc : LocalChain) : LocalChain :=
+      lc<|lc_contracts ::= FMap.add addr wc|>.
 
-  Definition set_contract_state
-             (addr : Address)
-             (state : SerializedValue)
-             (lc : LocalChain) : LocalChain :=
-    lc<|lc_contract_state ::= FMap.add addr state|>.
+    Definition set_contract_state
+                (addr : Address)
+                (state : SerializedValue)
+                (lc : LocalChain) : LocalChain :=
+      lc<|lc_contract_state ::= FMap.add addr state|>.
+    
+    Definition weak_error_to_error_init
+                (r : result SerializedValue SerializedValue)
+                : result SerializedValue ActionEvaluationError :=
+      bind_error (fun err => init_failed err) r.
 
-  Definition send_or_call
-             (origin : Address)
-             (from to : Address)
-             (amount : Amount)
-             (msg : option SerializedValue)
-             (lc : LocalChain) : result (list Action * LocalChain) ActionEvaluationError :=
-    do if amount <? 0 then Err amount_negative else Ok tt;
-    do if amount >? env_account_balances lc from then Err amount_too_high else Ok tt;
-    match FMap.find to lc.(lc_contracts) with
-    | None =>
-      (* Fail if sending a message to address without contract *)
-      do if address_is_contract to then Err no_such_contract else Ok tt;
-      match msg with
-        | None => Ok ([], transfer_balance from to amount lc)
-        | Some msg => Err no_such_contract
-      end
-    | Some wc =>
-      do state <- result_of_option (env_contract_states lc to) internal_error;
-      let lc := transfer_balance from to amount lc in
-      let ctx := build_ctx origin from to (env_account_balances lc to) amount in
-      do '(new_state, new_actions) <- result_of_option (wc_receive wc lc ctx state msg)
-                                                       receive_failed;
-      let lc := set_contract_state to new_state lc in
-      Ok (map (build_act origin to) new_actions, lc)
-    end.
+    Definition weak_error_to_error_receive
+                (r : result (SerializedValue * list ActionBody) SerializedValue)
+                : result (SerializedValue * list ActionBody) ActionEvaluationError :=
+      bind_error (fun err => receive_failed err) r.
 
-  Definition deploy_contract
-             (origin : Address)
-             (from : Address)
-             (amount : Amount)
-             (wc : WeakContract)
-             (setup : SerializedValue)
-             (lc : LocalChain)
-    : result (list Action * LocalChain) ActionEvaluationError :=
-    do if amount <? 0 then Err amount_negative else Ok tt;
-    do if amount >? env_account_balances lc from then Err amount_too_high else Ok tt;
-    do contract_addr <- result_of_option (get_new_contract_addr lc) too_many_contracts;
-    do match FMap.find contract_addr (lc_contracts lc) with
-       | Some _ => Err internal_error
-       | None => Ok tt
-       end;
-    let lc := transfer_balance from contract_addr amount lc in
-    let ctx := build_ctx origin from contract_addr amount amount in
-    do state <- result_of_option (wc_init wc lc ctx setup) init_failed;
-    let lc := add_contract contract_addr wc lc in
-    let lc := set_contract_state contract_addr state lc in
-    Ok ([], lc).
+    Definition send_or_call
+                (origin : Address)
+                (from to : Address)
+                (amount : Amount)
+                (msg : option SerializedValue)
+                (lc : LocalChain) : result (list Action * LocalChain) ActionEvaluationError :=
+      do if amount <? 0 then Err (amount_negative amount) else Ok tt;
+      do if amount >? env_account_balances lc from then Err (amount_too_high amount) else Ok tt;
+      match FMap.find to lc.(lc_contracts) with
+      | None =>
+        (* Fail if sending a message to address without contract *)
+        do if address_is_contract to then Err (no_such_contract to) else Ok tt;
+        match msg with
+          | None => Ok ([], transfer_balance from to amount lc)
+          | Some msg => Err (no_such_contract to)
+        end
+      | Some wc =>
+        do state <- result_of_option (env_contract_states lc to) internal_error;
+        let lc := transfer_balance from to amount lc in
+        let ctx := build_ctx origin from to (env_account_balances lc to) amount in
+        do '(new_state, new_actions) <- weak_error_to_error_receive (wc_receive wc lc ctx state msg);
+        let lc := set_contract_state to new_state lc in
+          Ok (map (build_act origin to) new_actions, lc)
+      end.
 
-  Local Open Scope nat.
+    Definition deploy_contract
+                (origin : Address)
+                (from : Address)
+                (amount : Amount)
+                (wc : WeakContract)
+                (setup : SerializedValue)
+                (lc : LocalChain)
+                : result (list Action * LocalChain) ActionEvaluationError :=
+      do if amount <? 0 then Err (amount_negative amount) else Ok tt;
+      do if amount >? env_account_balances lc from then Err (amount_too_high amount) else Ok tt;
+      do contract_addr <- result_of_option (get_new_contract_addr lc) too_many_contracts;
+      do match FMap.find contract_addr (lc_contracts lc) with
+        | Some _ => Err internal_error
+        | None => Ok tt
+        end;
+      let lc := transfer_balance from contract_addr amount lc in
+      let ctx := build_ctx origin from contract_addr amount amount in
+      do state <- weak_error_to_error_init (wc_init wc lc ctx setup);
+      let lc := add_contract contract_addr wc lc in
+      let lc := set_contract_state contract_addr state lc in
+      Ok ([], lc).
 
-  Definition execute_action (act : Action) (lc : LocalChain) :
-    result (list Action * LocalChain) ActionEvaluationError :=
-    match act with
-    | build_act origin from (act_transfer to amount) =>
-      send_or_call origin from to amount None lc
-    | build_act origin from (act_deploy amount wc setup) =>
-      deploy_contract origin from amount wc setup lc
-    | build_act origin from (act_call to amount msg) =>
-      send_or_call origin  from to amount (Some msg) lc
-    end.
+    Local Open Scope nat.
 
-  Fixpoint execute_actions
-           (count : nat)
-           (acts : list Action)
-           (lc : LocalChain)
-           (depth_first : bool)
-    : result LocalChain AddBlockError :=
-    match count, acts with
-    | _, [] => Ok lc
-    | 0, _ => Err action_evaluation_depth_exceeded
-    | S count, act :: acts =>
-      match execute_action act lc with
-      | Ok (next_acts, lc) =>
-        let acts := if depth_first
-                    then next_acts ++ acts
-                    else acts ++ next_acts in
-        execute_actions count acts lc depth_first
-      | Err act_err =>
-        Err (action_evaluation_error act act_err)
-      end
-    end.
+    Definition execute_action
+                (act : Action)
+                (lc : LocalChain)
+                : result (list Action * LocalChain) ActionEvaluationError :=
+      match act with
+      | build_act origin from (act_transfer to amount) =>
+        send_or_call origin from to amount None lc
+      | build_act origin from (act_deploy amount wc setup) =>
+        deploy_contract origin from amount wc setup lc
+      | build_act origin from (act_call to amount msg) =>
+        send_or_call origin  from to amount (Some msg) lc
+      end.
 
-  Lemma transfer_balance_equiv from to amount (lc : LocalChain) (env : Environment) :
-    EnvironmentEquiv lc env ->
-    EnvironmentEquiv
-      (transfer_balance from to amount lc)
-      (Blockchain.transfer_balance from to amount env).
+    Fixpoint execute_actions
+              (count : nat)
+              (acts : list Action)
+              (lc : LocalChain)
+              (depth_first : bool)
+              : result LocalChain AddBlockError :=
+      match count, acts with
+      | _, [] => Ok lc
+      | 0, _ => Err action_evaluation_depth_exceeded
+      | S count, act :: acts =>
+        match execute_action act lc with
+        | Ok (next_acts, lc) =>
+          let acts := if depth_first
+                      then next_acts ++ acts
+                      else acts ++ next_acts in
+          execute_actions count acts lc depth_first
+        | Err act_err =>
+          Err (action_evaluation_error act act_err)
+        end
+      end.
+
+    Lemma transfer_balance_equiv
+            (from to : Address)
+            (amount : Amount)
+            (lc : LocalChain)
+            (env : Environment) :
+      EnvironmentEquiv lc env ->
+      EnvironmentEquiv
+        (transfer_balance from to amount lc)
+        (Blockchain.transfer_balance from to amount env).
+    Proof.
+      intros <-.
+      apply build_env_equiv; auto.
+      cbn.
+      intros addr.
+      unfold Amount in *.
+      destruct_address_eq; subst;
+        repeat
+          (try rewrite FMap.find_partial_alter;
+          try rewrite FMap.find_partial_alter_ne by auto;
+          cbn); lia.
+    Defined.
+
+    Lemma set_contract_state_equiv addr state (lc : LocalChain) (env : Environment) :
+      EnvironmentEquiv lc env ->
+      EnvironmentEquiv
+        (set_contract_state addr state lc)
+        (Blockchain.set_contract_state addr state env).
+    Proof.
+      intros <-.
+      apply build_env_equiv; auto.
+      intros addr'.
+      cbn.
+      unfold set_chain_contract_state.
+      destruct_address_eq.
+      - subst. now rewrite FMap.find_add.
+      - rewrite FMap.find_add_ne; auto.
+    Defined.
+
+    Lemma add_contract_equiv addr wc (lc : LocalChain) (env : Environment) :
+      EnvironmentEquiv lc env ->
+      EnvironmentEquiv
+        (add_contract addr wc lc)
+        (Blockchain.add_contract addr wc env).
+    Proof.
+      intros <-.
+      apply build_env_equiv; auto.
+      intros addr'.
+      cbn.
+      destruct_address_eq.
+      - subst. now rewrite FMap.find_add.
+      - rewrite FMap.find_add_ne; auto.
+    Defined.
+
+    Local Open Scope Z.
+    Lemma gtb_le x y :
+      x >? y = false ->
+      x <= y.
+    Proof.
+      intros H.
+      rewrite Z.gtb_ltb in H.
+      apply Z.ltb_ge.
+      auto.
+    Defined.
+
+    Lemma ltb_ge x y :
+      x <? y = false ->
+      x >= y.
+    Proof.
+      intros H.
+      apply Z.ltb_ge in H.
+      lia.
+    Defined.
+
+    Local Hint Resolve gtb_le ltb_ge : core.
+
+    Lemma send_or_call_step origin from to amount msg act lc_before new_acts lc_after :
+      send_or_call origin from to amount msg lc_before = Ok (new_acts, lc_after) ->
+      act = build_act origin from (match msg with
+                                  | None => act_transfer to amount
+                                  | Some msg => act_call to amount msg
+                                  end) ->
+      ActionEvaluation lc_before act lc_after new_acts.
+    Proof.
+      intros sent act_eq.
+      unfold send_or_call in sent.
+      destruct (Z.ltb amount 0) eqn:amount_nonnegative;
+        [cbn in *; congruence|].
+      destruct (Z.gtb amount (env_account_balances lc_before from)) eqn:balance_enough;
+        [cbn in *; congruence|].
+      destruct (FMap.find to (lc_contracts lc_before)) as [wc|] eqn:to_contract.
+      - (* there is a contract at destination, so do call *)
+        destruct (env_contract_states _ _) as [prev_state|] eqn:prev_state_eq;
+          [|cbn in *; congruence].
+        cbn -[lc_to_env] in *.
+        destruct (wc_receive wc _ _ _ _) as [[new_state resp_acts]|] eqn:receive;
+          [|cbn in *; congruence].
+        apply (eval_call origin from to amount wc msg prev_state new_state resp_acts);
+          try solve [cbn in *; auto; congruence].
+        + cbn in sent.
+          inversion_clear sent.
+          rewrite <- receive.
+          auto.
+        + inversion sent; subst;
+            now apply set_contract_state_equiv, transfer_balance_equiv.
+      - (* no contract at destination, so msg should be empty *)
+        destruct (address_is_contract to) eqn:addr_format; cbn in *; try congruence.
+        destruct msg; cbn in *; try congruence.
+        assert (new_acts = []) by congruence; subst new_acts.
+        apply (eval_transfer origin from to amount); auto.
+        inversion sent; subst; now apply transfer_balance_equiv.
+    Defined.
+
+    Lemma get_new_contract_addr_is_contract_addr lc addr :
+      get_new_contract_addr lc = Some addr ->
+      address_is_contract addr = true.
+    Proof.
+      intros get.
+      unfold get_new_contract_addr in get.
+      pose proof (BoundedN.of_N_some get) as eq.
+      destruct addr as [addr prf].
+      cbn in *; rewrite eq.
+      match goal with
+      | [|- context[N.leb ?a ?b = true]] => destruct (N.leb_spec a b); auto; lia
+      end.
+    Defined.
+
+    Local Hint Resolve get_new_contract_addr_is_contract_addr : core.
+    Lemma deploy_contract_step origin from amount wc setup act lc_before new_acts lc_after :
+      deploy_contract origin from amount wc setup lc_before = Ok (new_acts, lc_after) ->
+      act = build_act origin from (act_deploy amount wc setup) ->
+      ActionEvaluation lc_before act lc_after new_acts.
+    Proof.
+      intros dep act_eq.
+      unfold deploy_contract in dep.
+      destruct (Z.ltb amount 0) eqn:amount_nonnegative;
+        [cbn in *; congruence|].
+      destruct (Z.gtb amount (env_account_balances lc_before from)) eqn:balance_enough;
+        [cbn in *; congruence|].
+      destruct (get_new_contract_addr lc_before) as [contract_addr|] eqn:new_contract_addr;
+        [|cbn in *; congruence].
+      cbn -[incoming_txs] in dep.
+      destruct (FMap.find _ _) eqn:no_contracts; [cbn in *; congruence|].
+      destruct (wc_init _ _ _ _) as [state|] eqn:recv; [|cbn in *; congruence].
+      cbn in dep.
+      assert (new_acts = []) by congruence; subst new_acts.
+      apply (eval_deploy origin from contract_addr amount wc setup state); eauto.
+      inversion dep; subst lc_after.
+      now apply set_contract_state_equiv, add_contract_equiv, transfer_balance_equiv.
+    Defined.
+
+    Local Hint Resolve send_or_call_step deploy_contract_step : core.
+    Lemma execute_action_step
+          (act : Action)
+          (new_acts : list Action)
+          (lc_before : LocalChain)
+          (lc_after : LocalChain) :
+      execute_action act lc_before = Ok (new_acts, lc_after) ->
+      ActionEvaluation lc_before act lc_after new_acts.
+    Proof.
+      intros exec.
+      unfold execute_action in exec.
+      destruct act as [orig from body].
+      destruct body as [to amount|to amount msg|amount wc setup]; eauto.
+    Defined.
+
+    Hint Constructors ChainStep : core.
+    Hint Constructors ChainedList : core.
+    Hint Unfold ChainTrace : core.
+
+    Lemma execute_actions_trace count acts (lc lc_final : LocalChain) df
+          (trace : ChainTrace empty_state (build_chain_state lc acts)) :
+      execute_actions count acts lc df = Ok lc_final ->
+      ChainTrace empty_state (build_chain_state lc_final []).
+    Proof.
+      revert acts lc lc_final trace.
+      induction count as [| count IH]; intros acts lc lc_final trace exec; cbn in *.
+      - destruct acts; congruence.
+      - destruct acts as [|x xs]; try congruence.
+        destruct (execute_action x lc) as [[new_acts lc_after]|] eqn:exec_once;
+          cbn in *; try congruence.
+        set (step := execute_action_step _ _ _ _ exec_once).
+        refine (IH _ _ _ _ exec).
+        destruct df.
+        + (* depth-first case *)
+          eauto.
+        + (* breadth-first case. Insert permute step. *)
+          assert (Permutation (new_acts ++ xs) (xs ++ new_acts)) by perm_simplify.
+          cut (ChainTrace
+                empty_state
+                (build_chain_state lc_after (new_acts ++ xs))); eauto.
+          intros.
+          econstructor; eauto.
+          constructor; eauto.
+          constructor; eauto.
+    Defined.
+  End ExecuteActions.
+
+  Definition lc_initial : LocalChain :=
+    {| lc_height := 0;
+      lc_slot := 0;
+      lc_fin_height := 0;
+      lc_account_balances := FMap.empty;
+      lc_contract_state := FMap.empty;
+      lc_contracts := FMap.empty; |}.
+
+  Record LocalChainBuilder :=
+    build_local_chain_builder {
+      lcb_lc : LocalChain;
+      lcb_trace : ChainTrace empty_state (build_chain_state lcb_lc []);
+    }.
+
+  Definition lcb_initial : LocalChainBuilder :=
+    {| lcb_lc := lc_initial; lcb_trace := clnil |}.
+
+  Definition validate_header (header : BlockHeader) (chain : Chain) : bool :=
+    (block_height header =? S (chain_height chain))
+    && (current_slot chain <? block_slot header)
+    && (finalized_height chain <=? block_finalized_height header)
+    && (block_finalized_height header <? block_height header)
+    && negb (address_is_contract (block_creator header))
+    && (block_reward header >=? 0)%Z.
+
+  Lemma validate_header_valid header chain :
+    validate_header header chain = true ->
+    IsValidNextBlock header chain.
   Proof.
-    intros <-.
-    apply build_env_equiv; auto.
-    cbn.
-    intros addr.
-    unfold Amount in *.
-    destruct_address_eq; subst;
-      repeat
-        (try rewrite FMap.find_partial_alter;
-         try rewrite FMap.find_partial_alter_ne by auto;
-         cbn); lia.
-  Defined.
-
-  Lemma set_contract_state_equiv addr state (lc : LocalChain) (env : Environment) :
-    EnvironmentEquiv lc env ->
-    EnvironmentEquiv
-      (set_contract_state addr state lc)
-      (Blockchain.set_contract_state addr state env).
-  Proof.
-    intros <-.
-    apply build_env_equiv; auto.
-    intros addr'.
-    cbn.
-    unfold set_chain_contract_state.
-    destruct_address_eq.
-    - subst. now rewrite FMap.find_add.
-    - rewrite FMap.find_add_ne; auto.
-  Defined.
-
-  Lemma add_contract_equiv addr wc (lc : LocalChain) (env : Environment) :
-    EnvironmentEquiv lc env ->
-    EnvironmentEquiv
-      (add_contract addr wc lc)
-      (Blockchain.add_contract addr wc env).
-  Proof.
-    intros <-.
-    apply build_env_equiv; auto.
-    intros addr'.
-    cbn.
-    destruct_address_eq.
-    - subst. now rewrite FMap.find_add.
-    - rewrite FMap.find_add_ne; auto.
-  Defined.
-
-  Local Open Scope Z.
-  Lemma gtb_le x y :
-    x >? y = false ->
-    x <= y.
-  Proof.
-    intros H.
-    rewrite Z.gtb_ltb in H.
-    apply Z.ltb_ge.
-    auto.
-  Defined.
-
-  Lemma ltb_ge x y :
-    x <? y = false ->
-    x >= y.
-  Proof.
-    intros H.
-    apply Z.ltb_ge in H.
+    intros valid.
+    unfold validate_header in valid.
+    repeat
+      (match goal with
+      | [H: context[Nat.eqb ?a ?b] |- _] => destruct (Nat.eqb_spec a b)
+      | [H: context[Nat.ltb ?a ?b] |- _] => destruct (Nat.ltb_spec a b)
+      | [H: context[Nat.leb ?a ?b] |- _] => destruct (Nat.leb_spec a b)
+      | [H: context[Z.geb ?a ?b] |- _] => destruct (Z.geb_spec a b)
+      end; [|repeat rewrite Bool.andb_false_r in valid; cbn in valid; congruence]).
+    destruct (negb (address_is_contract (block_creator header))) eqn:to_acc;
+      [|cbn in valid; congruence].
+    apply Bool.negb_true_iff in to_acc.
+    apply build_is_valid_next_block; cbn; auto.
     lia.
   Defined.
 
-  Local Hint Resolve gtb_le ltb_ge : core.
+  Definition find_origin_neq_from (actions : list Action) : option Action :=
+    find (fun act => negb (address_eqb (act_origin act) (act_from act))) actions.
 
-  Lemma send_or_call_step origin from to amount msg act lc_before new_acts lc_after :
-    send_or_call origin from to amount msg lc_before = Ok (new_acts, lc_after) ->
-    act = build_act origin from (match msg with
-                                 | None => act_transfer to amount
-                                 | Some msg => act_call to amount msg
-                                 end) ->
-    ActionEvaluation lc_before act lc_after new_acts.
+  Lemma validate_origin_neq_from_valid actions :
+    find_origin_neq_from actions = None ->
+    Forall (fun act => address_eqb (act_origin act) (act_from act) = true) actions.
   Proof.
-    intros sent act_eq.
-    unfold send_or_call in sent.
-    destruct (Z.ltb amount 0) eqn:amount_nonnegative;
-      [cbn in *; congruence|].
-    destruct (Z.gtb amount (env_account_balances lc_before from)) eqn:balance_enough;
-      [cbn in *; congruence|].
-    destruct (FMap.find to (lc_contracts lc_before)) as [wc|] eqn:to_contract.
-    - (* there is a contract at destination, so do call *)
-      destruct (env_contract_states _ _) as [prev_state|] eqn:prev_state_eq;
-        [|cbn in *; congruence].
-      cbn -[lc_to_env] in *.
-      destruct (wc_receive wc _ _ _ _) as [[new_state resp_acts]|] eqn:receive;
-        [|cbn in *; congruence].
-      apply (eval_call origin from to amount wc msg prev_state new_state resp_acts);
-        try solve [cbn in *; auto; congruence].
-      + cbn in sent.
-        inversion_clear sent.
-        rewrite <- receive.
-        auto.
-      + inversion sent; subst;
-          now apply set_contract_state_equiv, transfer_balance_equiv.
-    - (* no contract at destination, so msg should be empty *)
-      destruct (address_is_contract to) eqn:addr_format; cbn in *; try congruence.
-      destruct msg; cbn in *; try congruence.
-      assert (new_acts = []) by congruence; subst new_acts.
-      apply (eval_transfer origin from to amount); auto.
-      inversion sent; subst; now apply transfer_balance_equiv.
+    intros find_none.
+    unfold find_origin_neq_from in find_none.
+    specialize (List.find_none _ _ find_none) as all_nin.
+    cbn in *.
+    assert (all_nin0 : forall x, In x actions -> (act_origin x =? act_from x)%address = true).
+    { intros. now apply ssrbool.negbFE. }
+    now apply Forall_forall in all_nin0.
   Defined.
 
-  Lemma get_new_contract_addr_is_contract_addr lc addr :
-    get_new_contract_addr lc = Some addr ->
-    address_is_contract addr = true.
+  Definition find_invalid_root_action (actions : list Action) : option Action :=
+    find (fun act => address_is_contract (act_from act)) actions.
+
+  Lemma validate_actions_valid actions :
+    find_invalid_root_action actions = None ->
+    Forall (fun act => act_is_from_account act) actions.
   Proof.
-    intros get.
-    unfold get_new_contract_addr in get.
-    pose proof (BoundedN.of_N_some get) as eq.
-    destruct addr as [addr prf].
-    cbn in *; rewrite eq.
-    match goal with
-    | [|- context[N.leb ?a ?b = true]] => destruct (N.leb_spec a b); auto; lia
-    end.
+    intros find_none.
+    unfold find_invalid_root_action in find_none.
+    specialize (List.find_none _ _ find_none) as all_nin.
+    unfold act_is_from_account.
+    now apply Forall_forall in all_nin.
   Defined.
 
-  Local Hint Resolve get_new_contract_addr_is_contract_addr : core.
-  Lemma deploy_contract_step origin from amount wc setup act lc_before new_acts lc_after :
-    deploy_contract origin from amount wc setup lc_before = Ok (new_acts, lc_after) ->
-    act = build_act origin from (act_deploy amount wc setup) ->
-    ActionEvaluation lc_before act lc_after new_acts.
+  Definition add_new_block (header : BlockHeader) (lc : LocalChain) : LocalChain :=
+    let lc := add_balance (block_creator header) (block_reward header) lc in
+    lc<|lc_height := block_height header|>
+      <|lc_slot := block_slot header|>
+      <|lc_fin_height := block_finalized_height header|>.
+
+  Lemma add_new_block_equiv header (lc : LocalChain) (env : Environment) :
+    EnvironmentEquiv lc env ->
+    EnvironmentEquiv
+      (add_new_block header lc)
+      (Blockchain.add_new_block_to_env header env).
   Proof.
-    intros dep act_eq.
-    unfold deploy_contract in dep.
-    destruct (Z.ltb amount 0) eqn:amount_nonnegative;
-      [cbn in *; congruence|].
-    destruct (Z.gtb amount (env_account_balances lc_before from)) eqn:balance_enough;
-      [cbn in *; congruence|].
-    destruct (get_new_contract_addr lc_before) as [contract_addr|] eqn:new_contract_addr;
-      [|cbn in *; congruence].
-    cbn -[incoming_txs] in dep.
-    destruct (FMap.find _ _) eqn:no_contracts; [cbn in *; congruence|].
-    destruct (wc_init _ _ _ _) as [state|] eqn:recv; [|cbn in *; congruence].
-    cbn in dep.
-    assert (new_acts = []) by congruence; subst new_acts.
-    apply (eval_deploy origin from contract_addr amount wc setup state); eauto.
-    inversion dep; subst lc_after.
-    now apply set_contract_state_equiv, add_contract_equiv, transfer_balance_equiv.
-  Defined.
-
-  Local Hint Resolve send_or_call_step deploy_contract_step : core.
-  Lemma execute_action_step
-        (act : Action)
-        (new_acts : list Action)
-        (lc_before : LocalChain)
-        (lc_after : LocalChain) :
-    execute_action act lc_before = Ok (new_acts, lc_after) ->
-    ActionEvaluation lc_before act lc_after new_acts.
-  Proof.
-    intros exec.
-    unfold execute_action in exec.
-    destruct act as [orig from body].
-    destruct body as [to amount|to amount msg|amount wc setup]; eauto.
-  Defined.
-
-  Hint Constructors ChainStep : core.
-  Hint Constructors ChainedList : core.
-  Hint Unfold ChainTrace : core.
-
-  Lemma execute_actions_trace count acts (lc lc_final : LocalChain) df
-        (trace : ChainTrace empty_state (build_chain_state lc acts)) :
-    execute_actions count acts lc df = Ok lc_final ->
-    ChainTrace empty_state (build_chain_state lc_final []).
-  Proof.
-    revert acts lc lc_final trace.
-    induction count as [| count IH]; intros acts lc lc_final trace exec; cbn in *.
-    - destruct acts; congruence.
-    - destruct acts as [|x xs]; try congruence.
-      destruct (execute_action x lc) as [[new_acts lc_after]|] eqn:exec_once;
-        cbn in *; try congruence.
-      set (step := execute_action_step _ _ _ _ exec_once).
-      refine (IH _ _ _ _ exec).
-      destruct df.
-      + (* depth-first case *)
-        eauto.
-      + (* breadth-first case. Insert permute step. *)
-        assert (Permutation (new_acts ++ xs) (xs ++ new_acts)) by perm_simplify.
-        cut (ChainTrace
-              empty_state
-              (build_chain_state lc_after (new_acts ++ xs))); eauto.
-        intros.
-        econstructor; eauto.
-        constructor; eauto.
-        constructor; eauto.
-  Defined.
-End ExecuteActions.
-
-Definition lc_initial : LocalChain :=
-  {| lc_height := 0;
-     lc_slot := 0;
-     lc_fin_height := 0;
-     lc_account_balances := FMap.empty;
-     lc_contract_state := FMap.empty;
-     lc_contracts := FMap.empty; |}.
-
-Record LocalChainBuilder :=
-  build_local_chain_builder {
-    lcb_lc : LocalChain;
-    lcb_trace : ChainTrace empty_state (build_chain_state lcb_lc []);
-  }.
-
-Definition lcb_initial : LocalChainBuilder :=
-  {| lcb_lc := lc_initial; lcb_trace := clnil |}.
-
-Definition validate_header (header : BlockHeader) (chain : Chain) : bool :=
-  (block_height header =? S (chain_height chain))
-  && (current_slot chain <? block_slot header)
-  && (finalized_height chain <=? block_finalized_height header)
-  && (block_finalized_height header <? block_height header)
-  && negb (address_is_contract (block_creator header))
-  && (block_reward header >=? 0)%Z.
-
-Lemma validate_header_valid header chain :
-  validate_header header chain = true ->
-  IsValidNextBlock header chain.
-Proof.
-  intros valid.
-  unfold validate_header in valid.
-  repeat
-    (match goal with
-    | [H: context[Nat.eqb ?a ?b] |- _] => destruct (Nat.eqb_spec a b)
-    | [H: context[Nat.ltb ?a ?b] |- _] => destruct (Nat.ltb_spec a b)
-    | [H: context[Nat.leb ?a ?b] |- _] => destruct (Nat.leb_spec a b)
-    | [H: context[Z.geb ?a ?b] |- _] => destruct (Z.geb_spec a b)
-    end; [|repeat rewrite Bool.andb_false_r in valid; cbn in valid; congruence]).
-  destruct (negb (address_is_contract (block_creator header))) eqn:to_acc;
-    [|cbn in valid; congruence].
-  apply Bool.negb_true_iff in to_acc.
-  apply build_is_valid_next_block; cbn; auto.
-  lia.
-Defined.
-
-Definition find_origin_neq_from (actions : list Action) : option Action :=
-  find (fun act => negb (address_eqb (act_origin act) (act_from act))) actions.
-
-Lemma validate_origin_neq_from_valid actions :
-  find_origin_neq_from actions = None ->
-  Forall (fun act => address_eqb (act_origin act) (act_from act) = true) actions.
-Proof.
-  intros find_none.
-  unfold find_origin_neq_from in find_none.
-  specialize (List.find_none _ _ find_none) as all_nin.
-  cbn in *.
-  assert (all_nin0 : forall x, In x actions -> (act_origin x =? act_from x)%address = true).
-  { intros. now apply ssrbool.negbFE. }
-  now apply Forall_forall in all_nin0.
-Defined.
-
-Definition find_invalid_root_action (actions : list Action) : option Action :=
-  find (fun act => address_is_contract (act_from act)) actions.
-
-Lemma validate_actions_valid actions :
-  find_invalid_root_action actions = None ->
-  Forall (fun act => act_is_from_account act) actions.
-Proof.
-  intros find_none.
-  unfold find_invalid_root_action in find_none.
-  specialize (List.find_none _ _ find_none) as all_nin.
-  unfold act_is_from_account.
-  now apply Forall_forall in all_nin.
-Defined.
-
-Definition add_new_block (header : BlockHeader) (lc : LocalChain) : LocalChain :=
-  let lc := add_balance (block_creator header) (block_reward header) lc in
-  lc<|lc_height := block_height header|>
-    <|lc_slot := block_slot header|>
-    <|lc_fin_height := block_finalized_height header|>.
-
-Lemma add_new_block_equiv header (lc : LocalChain) (env : Environment) :
-  EnvironmentEquiv lc env ->
-  EnvironmentEquiv
-    (add_new_block header lc)
-    (Blockchain.add_new_block_to_env header env).
-Proof.
-  intros eq.
-  apply build_env_equiv; try apply eq; auto.
-  intros addr.
-  cbn.
-  unfold Blockchain.add_balance.
-  destruct_address_eq.
-  - subst. rewrite FMap.find_partial_alter.
+    intros eq.
+    apply build_env_equiv; try apply eq; auto.
+    intros addr.
     cbn.
-    f_equal.
-    apply eq.
-  - rewrite FMap.find_partial_alter_ne; auto.
-    apply eq.
-Defined.
+    unfold Blockchain.add_balance.
+    destruct_address_eq.
+    - subst. rewrite FMap.find_partial_alter.
+      cbn.
+      f_equal.
+      apply eq.
+    - rewrite FMap.find_partial_alter_ne; auto.
+      apply eq.
+  Defined.
 
-(* The computational bits of adding a block *)
-Definition add_block_exec
-           (depth_first : bool)
-           (lc : LocalChain)
-           (header : BlockHeader)
-           (actions : list Action) : result LocalChain AddBlockError :=
-  do (if validate_header header lc then Ok tt else Err invalid_header);
-  do (match find_origin_neq_from actions with
-      | Some act => Err (origin_from_mismatch act)
-      | None => Ok tt
-      end);
-  do (match find_invalid_root_action actions with
-      | Some act => Err (invalid_root_action act)
-      | None => Ok tt
-      end);
-  let lc := add_new_block header lc in
-  execute_actions 1000 actions lc depth_first.
+  (* The computational bits of adding a block *)
+  Definition add_block_exec
+            (depth_first : bool)
+            (lc : LocalChain)
+            (header : BlockHeader)
+            (actions : list Action) : result LocalChain AddBlockError :=
+    do (if validate_header header lc then Ok tt else Err (invalid_header header));
+    do (match find_origin_neq_from actions with
+        | Some act => Err (origin_from_mismatch act)
+        | None => Ok tt
+        end);
+    do (match find_invalid_root_action actions with
+        | Some act => Err (invalid_root_action act)
+        | None => Ok tt
+        end);
+    let lc := add_new_block header lc in
+    execute_actions 1000 actions lc depth_first.
 
-Local Hint Resolve validate_header_valid validate_actions_valid validate_origin_neq_from_valid : core.
+  Local Hint Resolve validate_header_valid validate_actions_valid validate_origin_neq_from_valid : core.
 
-(* Adds a block to the chain by executing the specified chain actions.
-   Returns the new chain if the execution succeeded (for instance,
-   transactions need enough funds, contracts should not reject, etc. *)
-Definition add_block
-           (depth_first : bool)
-           (lcb : LocalChainBuilder)
-           (header : BlockHeader)
-           (actions : list Action) : result LocalChainBuilder AddBlockError.
-Proof.
-  set (lcopt := add_block_exec depth_first (lcb_lc lcb) header actions).
-  unfold add_block_exec in lcopt.
-  destruct lcopt as [lc|e] eqn:exec; [|exact (Err e)].
-  subst lcopt.
-  destruct (validate_header _) eqn:validate; [|cbn in exec; congruence].
-  destruct (find_origin_neq_from _) eqn:no_origin_neq_from;[cbn in exec; congruence|].
-  destruct (find_invalid_root_action _) eqn:no_invalid_root_act; [cbn in exec; congruence|].
-  destruct lcb as [prev_lc_end prev_lcb_trace].
-  refine (Ok {| lcb_lc := lc; lcb_trace := _ |}).
-  cbn -[execute_actions] in exec.
+  (* Adds a block to the chain by executing the specified chain actions.
+    Returns the new chain if the execution succeeded (for instance,
+    transactions need enough funds, contracts should not reject, etc. *)
+  Definition add_block
+            (depth_first : bool)
+            (lcb : LocalChainBuilder)
+            (header : BlockHeader)
+            (actions : list Action) : result LocalChainBuilder AddBlockError.
+  Proof.
+    set (lcopt := add_block_exec depth_first (lcb_lc lcb) header actions).
+    unfold add_block_exec in lcopt.
+    destruct lcopt as [lc|e] eqn:exec; [|exact (Err e)].
+    subst lcopt.
+    destruct (validate_header _) eqn:validate; [|cbn in exec; congruence].
+    destruct (find_origin_neq_from _) eqn:no_origin_neq_from;[cbn in exec; congruence|].
+    destruct (find_invalid_root_action _) eqn:no_invalid_root_act; [cbn in exec; congruence|].
+    destruct lcb as [prev_lc_end prev_lcb_trace].
+    refine (Ok {| lcb_lc := lc; lcb_trace := _ |}).
+    cbn -[execute_actions] in exec.
 
-  refine (execute_actions_trace _ _ _ _ _ _ exec).
-  refine (snoc prev_lcb_trace _).
-  apply (step_block _ _ header); auto.
-  apply add_new_block_equiv.
-  reflexivity.
-Defined.
+    refine (execute_actions_trace _ _ _ _ _ _ exec).
+    refine (snoc prev_lcb_trace _).
+    apply (step_block _ _ header); auto.
+    apply add_new_block_equiv.
+    reflexivity.
+  Defined.
 
-Definition LocalChainBuilderImpl : ChainBuilderType :=
-  {| builder_type := LocalChainBuilder;
-     builder_initial := lcb_initial;
-     builder_env lcb := lcb_lc lcb;
-     builder_add_block := add_block DepthFirst;
-     builder_trace := lcb_trace; |}.
+  Definition LocalChainBuilderImpl : ChainBuilderType :=
+    {| builder_type := LocalChainBuilder;
+      builder_initial := lcb_initial;
+      builder_env lcb := lcb_lc lcb;
+      builder_add_block := add_block DepthFirst;
+      builder_trace := lcb_trace; |}.
 
 End LocalBlockchain.
 
